WIP on LM to TM for closing Cook-Theorem-Assumptions

theories/L/Complexity/Reductions/TMGenNP/LMGenNP.v
@@ -13,13 +13,20 @@ Section fixX.
   Local Unset Implicit Arguments.
   Context (X:Type) `{R__X : registered X}.   
 
+  Definition LMGenNP : list Tok*nat*nat -> Prop:= 
+               (fun '(P, maxSize, k (*in unary*)) =>
+                  exists (c:X), size (enc c) <= maxSize /\ (exists sigma k', k' <= k /\ evaluatesIn step k' (initLMGen P (compile (enc c))) sigma)).
+
+
+  
+  (* This subset is the one that is already NP-hard *)
   Definition LMHaltsOrDiverges : list Tok*nat*nat -> Prop :=
     fun '(P, maxSize, steps (*in unary*)) =>
       (exists s, P = compile s /\ proc s)
-      /\ forall (c : X), size (enc c) <= maxSize -> forall k sigma', evaluatesIn step k (initLMGen P (compile (enc c))) sigma' -> k <= steps.
+      /\ (forall (c:X) k sigma, evaluatesIn step k (initLMGen P (compile (enc c))) sigma
+                          -> exists (c':X)  sigma', size (enc c') <= maxSize
+                                            /\ star step (initLMGen P (compile (enc c'))) sigma')
+      /\ forall (c : X), size (enc c) <= maxSize -> forall k sigma, evaluatesIn step k (initLMGen P (compile (enc c))) sigma -> k <= steps.
 
-  Definition LMGenNP : list Tok*nat*nat -> Prop:= 
-               (fun '(P, maxSize, k (*in unary*)) =>
-                  exists (c:X), size (enc c) <= maxSize /\ (exists sigma' k', k' <= k /\ evaluatesIn step k' (initLMGen P (compile (enc c))) sigma')).
 End fixX.
 
