theories/L/Complexity/Problems/GenNP/GenNP.v
@@ -9,14 +9,22 @@ Import L_Notations.
 Section GenNP.
   Context (X__cert : Type) `{R__cert : registered X__cert}.
 
-  Definition LHaltsOrDiverges : term*nat*nat -> Prop :=
-    fun '(s, maxSize, steps (*in unary*)) =>
-      proc s /\ forall (c:X__cert), size (enc c) <= maxSize -> forall k t, s (enc c) ⇓(k) t -> k <= steps.
-
+  
   Definition GenNP : term*nat*nat -> Prop :=
                (fun '(s, maxSize, steps (*in unary*)) =>
                   exists (c:X__cert), size (enc c) <= maxSize
                                /\ exists t, app s (enc c) ⇓(<=steps) t).
+
+  
+  (* This subset is the one that is already NP-hard:
+  procedures such that:
+  - if any certificate is valid, then a small one is valid
+  - For small certificates, we do not need much time *)
+  Definition LHaltsOrDiverges : term*nat*nat -> Prop :=
+    fun '(s, maxSize, steps (*in unary*)) =>
+      proc s
+      /\ (forall (c:X__cert) k t, s (enc c) ⇓(k) t -> exists (c':X__cert), size (enc c') <= maxSize /\ s (enc c') ⇓ t)
+      /\ (forall (c:X__cert), size (enc c) <= maxSize -> forall k t, s (enc c) ⇓(k) t -> k <= steps).  
 
 End GenNP.
 
