theories/L/Complexity/Reductions/TMGenNP/LM_to_mTM.v
@@ -13,14 +13,58 @@ From Undecidability Require Import TMGenNP.M_LM2TM.
 
 Check LMtoTM.M.
 
-Import LSum.
+From Undecidability Require Import LSum.
 
 From Undecidability Require Import CompCode. 
 
 Import ProgrammingTools.
 
+Module TrueOrDiverge.
+  Import TM.TM ProgrammingTools CaseList CaseBool Code.Decode Code.DecodeList.
+
+  Section sec.
+  Variable (n:nat) (sig : finType) (M' : pTM sig bool n).
+
+  Definition M := If M' Nop Diverge.
+
+  Lemma Realises R' (H' : M' ⊨ R'):
+    M ⊨ (fun tin out => R' tin (true,snd out)).
+  Proof.
+    eapply Realise_monotone.
+    { eapply If_Realise. eassumption. now TM_Correct. now apply Diverge_Realise. }
+    hnf. intros x [[] y]. intros [H|H].
+    -cbn in H. destruct H as (?&?&<-). easy. 
+    -exfalso. cbn in H. firstorder.
+  Qed.
+
+  Import TM.
+  
+  Lemma TerminatesIn R' (HR' : M' ⊨ R') T' (HT' : projT1 M' ↓ T'):
+    projT1 M ↓ (fun tin k => T' tin (k-1) /\ 0 < k /\ forall tout, ~ R' tin (false,tout)).
+  Proof.
+    eapply TerminatesIn_monotone.
+    { eapply If_TerminatesIn. 1,2:eassumption. now TM_Correct. now apply Canonical_TerminatesIn. }
+    intros tin [] (HTtin&Hfalse). easy. 
+    do 2 eexists;repeat simple apply conj. eassumption.
+    2:{ intros ? ? ?. destruct b. reflexivity. now exfalso. }
+    nia.
+  Qed.
+  End sec.
+End TrueOrDiverge.
+
+
 Arguments LMtoTM.M : clear implicits.
 
+
+(*move*)
+Lemma uniform_confluent_confluent (X : Type) (R : X -> X -> Prop):
+  uniform_confluent R -> confluent R.
+Proof.
+  intros H x y y' Hy Hy'. apply ARS.star_pow in Hy as (?&Hy). apply ARS.star_pow in Hy' as (?&Hy'). 
+  edestruct parametrized_confluence as (?&?&z&?&?&?&?&?).
+  eassumption. exact Hy. exact Hy'. exists z. split;eapply pow_star. all:easy.
+Qed. 
+  
 Lemma LMGenNP_to_TMGenNP_mTM :
   {sig : finType &
    {n:nat &
@@ -30,7 +74,7 @@ Lemma LMGenNP_to_TMGenNP_mTM :
 Proof.
   evar (sig : finType). evar (tau : finType). evar (n:nat).
   unshelve epose (_:mTM tau (S n)) as M.
-  { unshelve notypeclasses refine (projT1 (@LMtoTM.M sig _ _)).
+  { unshelve notypeclasses refine (projT1 ( (*TrueOrDiverge.M*) (@LMtoTM.M sig _ _))).
     2:now notypeclasses refine (Retract_inl _ (Retract_id _)).
     now notypeclasses refine (Retract_inr _ (Retract_id _)).
   } cbn in M.
@@ -50,8 +94,9 @@ Proof.
       (f:=fun '(P,maxSize,steps) => (ts__start P,f__size maxSize,f__steps steps P maxSize));subst tmp2;subst tmp3.
   2:{
     intros [[P maxSize] steps] H. split.
-    { hnf in H|-*. destruct H as ((s&Hs&s__proc)&Hk).
+    { hnf in H|-*. destruct H as ((s&Hs&s__proc)&HsmallCert&Hk).
       intros t__cert Hsize k conf__res HM.
+      
       apply LMtoTM.Realises in HM as HM__sound. hnf in HM__sound. specialize (HM__sound P).
       Tactic Notation "mp" hyp(L) "as" ident(H) :=
         lazymatch type of L with
@@ -72,10 +117,11 @@ Proof.
       2:{ erewrite loop_injective with (b:=conf__res). 3:exact HM__terminate. 2:eassumption.
           eassumption.
       }
+      cbn -[ts__start] in HMP.
       hnf.
       exists P. 
       set (t__M := f__UpToC _) at 1.
-      cut (forall steps__LM, steps__LM <= steps ->
+      cut (forall steps__LM, steps__LM <= steps -> 
                       t__M (steps__LM, sizeOfmTapes (t__cert ::: ts__start P)) <= f__steps steps P maxSize).
       {
         intros Hmono.
@@ -86,22 +132,67 @@ Proof.
             -left. split. 2:easy. eassumption.
             -apply Hmono. clear;nia. 
         }
-        edestruct HM__sound as (bs&?&?&k'&?).
-        { eexists k'. repeat simple apply conj.
+        edestruct HM__sound as (bs&?&?&k0&?).
+        cbn in H.
+        specialize sizeOfTape_tape_contains_size with (1:=tape_contains_contains_size H) as Hsize_bs.
+        set (tmp := sizeOfTape _) in Hsize,Hsize_bs. rewrite <- Hsize_bs in Hsize at 1. clear Hsize_bs tmp.
+
+        { (*specialize HsmallCert with (1:=H0) as (cert'&sigma'&Hcert'size&(k'&Hcert'R)%(proj1 (@ARS.star_pow _ _ _ _))). *)
+         eexists k0. repeat simple apply conj.
           -exact HMP.
           -exact HMright.
           -right. eauto.
-          -apply Hmono. eapply Hk. 2:eassumption.
-           (*TODO: Why is bs small? is it small? *Or do we need to check smallness somewhere? *)
-           admit.
+          -apply Hmono.
+           (*specialize HsmallCert with (1:=H0) as (cert'&sigma'&Hcert'size&Hcert'R).
+           replace x with sigma' in *.
+           2:{
+             eapply ARS.unique_normal_forms with (R:= LM_heap_def.step).
+             -eapply uniform_confluent_confluent,functional_uc, LM_heap_def.step_functional.
+             -destruct H0 as (H0'&?). apply pow_star,star_ecl in H0'. apply star_ecl in Hcert'R. rewrite <- H0',<-Hcert'R.
+           destruct (HsmallCert _ _ _H0) *)
+           eapply Hk. 2:eassumption.
+           Set Nested Proofs Allowed.
+           (*move*)
+           Lemma size_rev X {_:registered X} (xs : list X): L.size (enc (rev xs)) = L.size (enc xs).
+           Proof.
+             rewrite !size_list,map_rev,<- sumn_rev. easy.
+           Qed.
+
+           rewrite size_rev.
+           
+           (*move*)
+           Lemma Lsize_list_bool_le:
+             (fun (bs : list bool) => L.size (enc bs)) <=c (fun bs => length bs + 1).
+           Admitted.
+           Lemma length_le_TMsize_list_bool:
+             (fun (bs : list bool) => length bs + 1) <=c size.
+           Admitted.
+           specialize @correct__leUpToC with (l:=Lsize_list_bool_le) (x:=bs) as ->.
+           specialize @correct__leUpToC with (l:=length_le_TMsize_list_bool) (x:=bs) as ->.
+           rewrite Hsize.
+           rewrite <- mult_assoc_reverse.
+           set (c:= c__leUpToC * c__leUpToC).
+           enough (Hdiv:f__size maxSize <= maxSize / (c+1)).
+           { unshelve erewrite (_ : c <= c +1) at 1. clear;nia.
+             rewrite Hdiv,Nat.mul_div_le. 2:clear;nia. reflexivity.
+           }
+           [f__size]:refine (fun n => _). subst f__size;cbn beta. reflexivity.
         }
       }
       (* TODO: instantiate using monotonic property? *)
+      Import String. instantiate (f__steps := TODO ("above, and abstract important properties")).
       admit. 
     }
     (* TODO: We might canc opy some reasoning from the first part down here*)
-    admit.
-    (* (The hard hald) *)
+    (* TODO: do we need HsmallCert? *)
+    destruct H as ((s&->&s__proc)&HsmallCert&Hk).
+    unfold LMGenNP, TMGenNP_fixed_mTM.
+    split.
+    -intros (cert & HcertSize & sigma & k' &Hk' &HR'). admit.
+     
+    -admit. 
+  }
+  admit.
 Admitted.
 
 Print Assumptions LMGenNP_to_TMGenNP_mTM.
